Support predicated loads and stores

driver/VericertDriver.ml
@@ -96,7 +96,7 @@ let compile_c_file sourcename ifile ofile =
   end else begin
     let verilog =
       let translation = if !option_hls_schedule
-                        then Vericert.Compiler0.transf_hls_temp
+                        then Vericert.Compiler0.transf_hls
                         else Vericert.Compiler0.transf_hls
       in
       (* let _ = Vericert.Smtpredicate.check_smt (Vericert.Predicate0.Pimp ((Vericert.Predicate0.Pbase (Vericert.Camlcoq.P.of_int 2)),(Vericert.Predicate0.Pbase (Vericert.Camlcoq.P.of_int 2)))) in *)
